verified/Sets.dfy
@@ -1,0 +1,32 @@
+// lifted from ironfleet/src/Dafny/Distributed/Common/Collections/Sets.i.dfy
+
+function SetOfNumbersInRightExclusiveRange(a:int, b:int):set<int>
+    requires a <= b;
+    ensures forall opn :: a <= opn < b ==> opn in SetOfNumbersInRightExclusiveRange(a, b);
+    ensures forall opn :: opn in SetOfNumbersInRightExclusiveRange(a, b) ==> a <= opn < b;
+    ensures |SetOfNumbersInRightExclusiveRange(a, b)| == b-a;
+    decreases b-a;
+{
+    if a == b then {} else {a} + SetOfNumbersInRightExclusiveRange(a+1, b)
+}
+
+lemma ThingsIKnowAboutSubset<T>(x:set<T>, y:set<T>)
+    requires x<y;
+    ensures |x|<|y|;
+{
+    if (x!={}) {
+        var e :| e in x;
+        ThingsIKnowAboutSubset(x-{e}, y-{e});
+    }
+}
+
+lemma SubsetCardinality<T>(x:set<T>, y:set<T>)
+    ensures x<y ==> |x|<|y|;
+    ensures x<=y ==> |x|<=|y|;
+{
+    if (x<y) {
+        ThingsIKnowAboutSubset(x, y);
+    }
+    if (x==y) { // OBSERVE the other case
+    }
+}
